coq/proof/SoundPostcondCmd.v
@@ -17,7 +17,6 @@ Import Opsem.
 Require Import TODO.
 Require Import Validator.
 Require Import GenericValues.
-Require Import SimulationLocal.
 Require InvMem.
 Require InvState.
 Require Import SoundBase.
@@ -32,6 +31,14 @@ Lemma has_false_False
   False.
 Proof.
 Admitted.
+
+Lemma postcond_cmd_is_call
+      c_src c_tgt inv1 inv2
+      (POSTCOND: Postcond.postcond_cmd c_src c_tgt inv1 = Some inv2):
+  Instruction.isCallInst c_src = Instruction.isCallInst c_tgt.
+Proof.
+  destruct c_src, c_tgt; ss.
+Qed.
 
 (* TODO: we can assume source's progress *)
 (* TODO: we need to split the cases: call and non-call. *)
